src/Minimal.DICE.fst
@@ -12,94 +12,238 @@ module I  = FStar.Integers
 module HI  = Lib.IntTypes
 
 module SHA2= Hacl.Hash.SHA2
+module HMAC= Hacl.HMAC
 
 module B   = LowStar.Buffer
 module M   = LowStar.Modifies
 module HS  = FStar.HyperStack
 module HST = FStar.HyperStack.ST
+module IB  = LowStar.ImmutableBuffer
 
 /// Hash algorithm for dice
 let _DICE_ALG = SHA2_256
 
 /// Length of UDS for dice
-let _DICE_UDS_LENGTH   : I.uint_32 = 0x20
+let _DICE_UDS_LENGTH   : I.uint_32 = 0x20ul
 
 /// Length of hash digest for dice
 let _DICE_DIGEST_LENGTH: I.uint_32 = hash_len _DICE_ALG
 
+/// <><><><><><><><><><><><><> Global Buffers <><><><><><><><><><><><><><><><>
+
+///
+/// A global secret eternal `uds` buffer
+///
+/// NOTE: We use `gcmalloc` to alloca "eternal" `uds` buffer, which must live (have property `recallable`), instead of using `malloc` to alloca "freeale" buffer, which can be hand-managed (have property `freeable`)
+///
+/// FIXME: Should I allocate them in a `main` function with `HST.ST` effect and then invoke `diceStart`? *)
+///
+/// FIXME: Must hand-retain the `recallable` property?
+///
+/// FIXME: Top-level let-bindings should have `Tot` effect, which may wipe properties like disjointness?
+
+let uds
+  : (b: B.buffer uint8 {B.length b = v _DICE_UDS_LENGTH /\ B.recallable b})
+= B.gcmalloc HS.root (u8 0x00) _DICE_UDS_LENGTH
+
+///
+/// A global public eternal `measurement` buffer
+
+let measurement
+  : (b: hash_t _DICE_ALG {B.recallable b})
+= B.gcmalloc HS.root (u8 0x00) _DICE_DIGEST_LENGTH
+
+///
+/// A global secret eternal `cdi` buffer
+
+let cdi
+  : (b: hash_t _DICE_ALG {B.recallable b})
+= B.gcmalloc HS.root (u8 0x00) _DICE_DIGEST_LENGTH
+
+/// <><><><><><><><><><><><> H/W API <><><><><><><><><><><><><><><><>
+
+assume val uds_ghost: Ghost.erased (Seq.seq uint8)
+
+///
+/// H/W API which tells us whether the access of (H/W?) uds is disabled.
+/// FIXME: How to define this?
+assume val uds_is_disabled : Type0
+
+assume val init_uds
+  (u: unit)
+: HST.Stack unit
+  (requires fun h ->
+    (* `uds` lives in h *)
+      B.all_live h [B.buf uds]
+    (* global buffers disjoint *)
+    /\ B.all_disjoint [B.loc_buffer uds
+                     ;B.loc_buffer measurement
+                     ;B.loc_buffer cdi]
+    )
+  (ensures  fun h0 _ h1 ->
+    (* only `uds` buffer is modified *)
+      B.modifies (B.loc_buffer uds) h0 h1
+    (* get the right `uds` *)
+    (* FIXME: should I use `Ghost.reveal` here? *)
+    /\ B.as_seq h1 uds == Ghost.reveal uds_ghost)
+
+///
+/// Data used to wipe `uds`
+
+assume val irrelContent_as_list: list uint8
+let irrelContent = Seq.seq_of_list irrelContent_as_list
+
+///
+/// API to wipe `uds` buffer and disable uds access.
+
+assume val clear_and_disabled_uds
+  (u: unit)
+: HST.Stack unit
+  (requires fun h ->
+    (* `uds` lives in h *)
+      B.all_live h [B.buf uds]
+    (* global buffers disjoint *)
+    /\ B.all_disjoint [B.loc_buffer uds
+                     ;B.loc_buffer measurement
+                     ;B.loc_buffer cdi]
+    )
+  (ensures  fun h0 _ h1 ->
+    (* wiped `uds` buffer using some irrelevant content *)
+      B.as_seq h1 uds == irrelContent
+    (* the access of uds is disabled *)
+    /\ uds_is_disabled
+    (* only `uds` buffer is modified *)
+    /\ B.modifies (B.loc_buffer uds) h0 h1)
+
 /// <><><><><><><><><><><><><> DICE Stubs <><><><><><><><><><><><><><><><>
 
-/// Abstract API to get `UDS`
-assume val get_UDS
-  (size: nat)
-: HST.St (b:B.buffer HI.uint8 {B.length b = size})
-
-/// Abstract API to get `measurement` of RIoT
-assume val get_measurement
-  (alg: hash_alg)
-: HST.St (hash_t alg)
-
-/// Abstract SHA2 256 hash API
-assume val diceSHA256
-  (size : nat)
-  (data: B.lbuffer HI.uint8 size)
-  (digest: hash_t _DICE_ALG)
-: HST.St unit
-
-/// Abstract SHA2 256 API, which takes two input datas
-assume val diceSHA256_2
-  (size1 : nat)
-  (data1: B.lbuffer HI.uint8 size1)
-  (size2 : nat)
-  (data2 : B.lbuffer HI.uint8 size2)
-  (digest: hash_t _DICE_ALG)
-: HST.St unit
-
 ///
-/// <><><><><><><><><><><><> DICE Core main funtion <><><><><><><><><><><>
-///
-/// DICE main function, which
-/// 1. get `UDS` and `measurement` using API
-/// 2. computes `CDI` and return it
-/// 
-let diceStart ()
-: HST.Stack (B.lbuffer HI.uint8 (v _DICE_DIGEST_LENGTH))
-  (requires fun _ -> True)
-  (ensures  fun _ _ _ -> True)
+/// Compute `measurement`
+
+let compute_measurement
+  (riot_size: uint_32)
+  (riot_binary: B.buffer uint8 {B.len riot_binary = riot_size})
+: HST.Stack unit
+  (requires fun h ->
+    (* all buffers live in `h` *)
+      B.all_live h [B.buf uds
+                   ;B.buf measurement
+                   ;B.buf cdi
+                   ;B.buf riot_binary]
+    (* all buffers disjoint *)
+    /\ B.all_disjoint [B.loc_buffer uds
+                     ;B.loc_buffer measurement
+                     ;B.loc_buffer cdi
+                     ;B.loc_buffer riot_binary]
+    (* the length of `riot_binary` not exceeds the max input length of `SHA2.hash_256` *)
+    /\ B.length riot_binary <= max_input_length SHA2_256
+    )
+  (ensures  fun h0 _ h1 ->
+    (* only `measurement` buffer is modified *)
+      B.modifies (B.loc_buffer measurement) h0 h1
+    (* functional specification, actually already carried by `SHA2.hash_256` *)
+    /\ B.as_seq h1 measurement
+      == Spec.Agile.Hash.hash SHA2_256 (B.as_seq h0 riot_binary)
+    )
 =
-  HST.push_frame();
+  SHA2.hash_256
+    riot_binary
+    riot_size
+    measurement
 
-/// Get `uds` and `measurement` using API
-  let uds : B.lbuffer HI.uint8 _DICE_UDS_LENGTH = get_UDS (v _DICE_UDS_LENGTH) in
-  let measurement: hash_t _DICE_ALG = get_measurement _DICE_ALG in
+let uds_is_initialized h: Type0
+=
+  B.as_seq h uds == Ghost.reveal uds_ghost
 
-/// Allocate digests and `cdi`
-  let uDigest :hash_t _DICE_ALG = B.alloca (HI.u8 0x00) _DICE_DIGEST_LENGTH in
-  let rDigest :hash_t _DICE_ALG = B.alloca (HI.u8 0x00) _DICE_DIGEST_LENGTH in
-  let cdi: hash_t _DICE_ALG = B.alloca (HI.u8 0x00) _DICE_DIGEST_LENGTH in
+///
+/// Compute `cdi`
 
-/// Compute digest `uDigest` of `uds`
-    SHA2.hash_256
-      uds
-      _DICE_UDS_LENGTH
-      uDigest;
+let compute_cdi
+  (riot_size: uint_32)
+  (riot_binary: B.buffer uint8 {B.len riot_binary = riot_size})
+: HST.Stack unit
+  (requires fun h ->
+    (* all buffers live in `h` *)
+      B.all_live h [B.buf uds
+                   ;B.buf measurement
+                   ;B.buf cdi
+                   ;B.buf riot_binary]
+    (* all buffers disjoint *)
+    /\ B.all_disjoint [B.loc_buffer uds
+                     ;B.loc_buffer measurement
+                     ;B.loc_buffer cdi
+                     ;B.loc_buffer riot_binary]
+    (* the length of `riot_binary` not exceeds the max input length of `SHA2.hash_256` *)
+    /\ B.length riot_binary <= max_input_length SHA2_256
+    (* `uds` buffer is initialized *)
+    /\ uds_is_initialized h
+    )
+  (ensures  fun h0 _ h1 ->
+    (* only `measurement` buffer is modified *)
+      B.modifies (B.loc_union_l [B.loc_buffer measurement
+                                ;B.loc_buffer cdi]) h0 h1
+    )
+=
+  compute_measurement riot_size riot_binary;
+  HMAC.compute_sha2_256
+    cdi
+    uds         _DICE_UDS_LENGTH
+    measurement _DICE_DIGEST_LENGTH
 
-/// compute digest `rDigest` of `measurement`
-    diceSHA256
-      (v _DICE_DIGEST_LENGTH) measurement
-      rDigest;
 
-/// compute `cdi` from `uDigest` and `rDigest`
-    diceSHA256_2
-     (v _DICE_DIGEST_LENGTH) uDigest
-     (v _DICE_DIGEST_LENGTH) rDigest
-     cdi;
+/// <><><><><><><><><><><><> DICE main funtion <><><><><><><><><><><>
 
-/// Zero-out `uDigest` and `rDigest`
-    B.fill uDigest (HI.u8 0x00) _DICE_DIGEST_LENGTH;
-    B.fill rDigest (HI.u8 0x00) _DICE_DIGEST_LENGTH;
+let dice_main
+  (riot_size: uint_32)
+  (riot_binary: B.buffer uint8 {B.len riot_binary = riot_size})
+: HST.Stack unit
+  (requires fun h ->
+    (* all buffers live in `h` *)
+      B.all_live h [B.buf riot_binary]
+    (* all buffers disjoint *)
+    (* FIXME: How to retain or prove the disjointness of global buffers? *)
+    /\ B.all_disjoint [B.loc_buffer uds
+                     ;B.loc_buffer measurement
+                     ;B.loc_buffer cdi
+                     ;B.loc_buffer riot_binary]
+    (* the length of `riot_binary` not exceeds the max input length of `SHA2.hash_256` *)
+    /\ B.length riot_binary <= max_input_length SHA2_256
+    )
+  (ensures  fun h0 _ h1 -> True)
+=
+  (* retain liveness of global buffers *)
+  B.recall uds;
+  B.recall measurement;
+  B.recall cdi;
 
-  HST.pop_frame();
+  (* initialize `uds` *)
+  init_uds ();
 
-/// return `cdi`
-  cdi
+  (* compute `measurement` and `cdi` *)
+  compute_cdi
+    riot_size
+    riot_binary;
+
+  (* wipe `uds` buffer and disable uds access *)
+  clear_and_disabled_uds ()
+
+  // riot_main ()
+
+/// <><><><><><><><><><><><> C main funtion <><><><><><><><><><><>
+
+assume val riot_size: (i: uint_32 {v i <= max_input_length SHA2_256})
+assume val riot_binary: (b: B.buffer uint8 {B.length b = v riot_size})
+
+let main ()
+: HST.St C.exit_code
+=
+  let h = HST.get () in
+  assume (B.live h riot_binary);
+  assume (B.all_disjoint [B.loc_buffer uds
+                         ;B.loc_buffer measurement
+                         ;B.loc_buffer cdi
+                         ;B.loc_buffer riot_binary]);
+  dice_main
+    riot_size
+    riot_binary;
+  C.EXIT_SUCCESS
