Makefile
@@ -1,1 +1,4 @@
 include src/Makefile
+
+clean:
+	rm ./out/*
